refactored/shortened proofs and updated for 8.12

src/Arithmetic/Inv.v
@@ -22,6 +22,9 @@ Require Import Crypto.Util.ZUtil.Div.
 Require Import Crypto.Util.ZUtil.Lor.
 Require Import Crypto.Util.ZUtil.Land.
 Require Import Crypto.Util.ZUtil.ArithmeticShiftr.
+Require Import Crypto.Util.ZUtil.TwosComplement.
+Require Import Crypto.Util.ZUtil.SignBit.
+Require Import Crypto.Util.ZUtil.Pow.
 
 Import Positional.
 Import ListNotations.
@@ -39,13 +42,9 @@ Local Open Scope Z_scope.
 (**Definitions *)
 (************* *)
 
-(*twos complement evaluation *)
-Notation twosc m a :=
-  (if ((a mod 2 ^ m) <? 2 ^ (m - 1)) then a mod 2 ^ m else a mod 2 ^ m - 2 ^ m).
-
-(*Custom evaluation function for multi-limbg twos complement *)
-Definition eval_twosc machine_wordsize n f :=
-  twosc (machine_wordsize * Z.of_nat n) (eval (uweight machine_wordsize) n f).
+(*Evaluation function for multi-limb integers in twos complement *)
+Definition eval_twos_complement machine_wordsize n f :=
+  Z.twos_complement (machine_wordsize * Z.of_nat n) (eval (uweight machine_wordsize) n f).
 
 (*Saturated addition of multi-limb integers *)
 Local Definition sat_add machine_wordsize n f g :=
@@ -62,14 +61,14 @@ Definition sat_shiftr machine_wordsize n f :=
     (seq 0 (n - 1))) ++ [(nth_default 0 f (n - 1)) >> 1].
 
 (* arithmetic right shift of saturated multi-limb integers *)
-Definition sat_arithmetic_shiftr machine_wordsize n f :=
+Definition sat_arithmetic_shiftr1 machine_wordsize n f :=
   (map
      (fun i =>
         ((nth_default 0 f i) >> 1) |' (Z.truncating_shiftl machine_wordsize
                                                     (nth_default 0 f (i + 1))
                                                     (machine_wordsize - 1)))
      (seq 0 (n - 1)))
-    ++ [Z.arithmetic_shiftr machine_wordsize (nth_default 0 f (n - 1))].
+    ++ [Z.arithmetic_shiftr1 machine_wordsize (nth_default 0 f (n - 1))].
 
 (* Multi-limb parity check *)
 Definition sat_mod2 f :=
@@ -84,62 +83,10 @@ Definition sat_opp machine_wordsize n f :=
 
 Definition sat_zero n :=
   zeros n.
-  (* encode_no_reduce (uweight machine_wordsize) n 0. *)
-
-(************************************************* *)
-(**Lemmas about the twos complement representation *)
-(************************************************* *)
-
-Lemma twosc_one m (Hm : 1 < m) :
-  twosc m 1 = 1.
-Proof.
-  assert (1 < 2 ^ m) by (apply Zpow_facts.Zpower_gt_1; lia).
-  assert (1 < 2 ^ (m - 1)) by (apply Zpow_facts.Zpower_gt_1; lia).
-  apply Z.ltb_lt in H0. rewrite Z.mod_small, H0; lia. Qed.
-
-Lemma twosc_zero m (Hm : 0 < m):
-  twosc m 0 = 0.
-Proof.
-  assert (0 <? 2 ^ (m - 1) = true).
-  apply Z.ltb_lt; auto with zarith.
-  rewrite Z.mod_0_l by auto with zarith.
-  rewrite H; reflexivity. Qed.
-
-Lemma twosc_mod a m (Hm : 0 < m) :
-  twosc m (a mod 2 ^ m) = twosc m a.
-Proof. rewrite Z.mod_mod; try apply Z.pow_nonzero; lia. Qed.
-
-Lemma twosc_odd m a (Hm : 0 < m) : Z.odd (twosc m a) = Z.odd a.
-Proof.
-  destruct (a mod 2 ^m <? 2 ^ (m - 1));
-    simpl;
-    [ | unfold Z.sub; rewrite Z.odd_add_even];
-    rewrite ?Zodd_mod, <- ?(Znumtheory.Zmod_div_mod);
-    try (apply Z.pow_pos_nonneg; lia);
-    try (apply Zpow_facts.Zpower_divide; lia);
-    try reflexivity.
-  apply Z.even_spec. rewrite Z.even_opp, Z.even_pow; try lia; reflexivity. Qed.
-
-Lemma twosc_mod2 m a (Hm : 0 < m) : twosc m a mod 2 = a mod 2.
-Proof. rewrite Zmod_odd, twosc_odd, <- Zmod_odd by lia. reflexivity. Qed.
-
-Lemma twosc_bounds a m (Hm : 0 < m) :
-  - 2 ^ (m - 1) <= twosc m a < 2 ^ (m - 1).
-Proof.
-  assert (0 < 2 ^ m) by (apply Z.pow_pos_nonneg; lia).
-  assert (2 ^ m = 2 * 2 ^ (m - 1))
-    by (rewrite Pow.Z.pow_mul_base, Z.sub_simpl_r; lia).
-  pose proof (Z.mod_pos_bound a (2 ^ m) H).
-  destruct (a mod 2 ^ m <? 2 ^ (m - 1)) eqn:E.
-  - rewrite Z.ltb_lt in E; lia.
-  - apply Z.ltb_ge in E; lia. Qed.
 
 (*********************************************************************** *)
 (**Section for small independent lemmas which do not fit anywhere else   *)
 (*********************************************************************** *)
-
-Lemma app_split {A} (a b c d : list A) : a = c -> b = d -> a ++ b = c ++ d.
-Proof. now intros; subst. Qed.
 
 Lemma eval_bound machine_wordsize n f
       (mw0 : 0 < machine_wordsize)
@@ -159,19 +106,6 @@ Proof.
         (machine_wordsize + machine_wordsize * Z.of_nat (length f)) by nia.
       rewrite Z.pow_add_r; nia. Qed.
 
-Lemma mod_less_than_half_iff_not_neg_mod_less a m
-        (Hm : 0 < m)
-        (Ha1 : a mod 2 ^ m <> 2 ^ (m - 1))
-        (Ha2 : a mod 2 ^ m <> 0) :
-  (a mod 2 ^ m <? 2 ^ (m - 1)) = negb ((- a) mod 2 ^ m <? 2 ^ (m - 1)).
-Proof.
-  assert (0 < 2 ^ m) by (apply Z.pow_pos_nonneg; lia).
-  assert (a mod 2 ^ m + (- a mod 2 ^ m) = 2 * 2 ^ (m - 1)) by
-      (rewrite !Zmod_eq, Z_div_nz_opp_full, Pow.Z.pow_mul_base, Z.sub_simpl_r by lia; ring).
-  destruct (a mod 2 ^ m <? 2 ^ (m - 1)) eqn:E1;
-    destruct (- a mod 2 ^ m <? 2 ^ (m - 1)) eqn:E2;
-    rewrite ?Z.ltb_lt, ?Z.ltb_ge in *; try reflexivity; lia. Qed.
-
 (****************************************************************************** *)
 (**Section for lemma relating to bitwise operations and the Z.testbits function *)
 (****************************************************************************** *)
@@ -186,8 +120,10 @@ Lemma eval_testbit machine_wordsize n f m
 Proof.
   generalize dependent n. generalize dependent m. induction f; intros; simpl in *; subst.
   - rewrite ListUtil.nth_default_nil, eval0, !Z.testbit_0_l; reflexivity.
-  - rewrite eval_cons, uweight_eval_shift by lia.
-    rewrite uweight_0, uweight_eq_alt', Z.mul_1_l, Z.mul_1_r, Z.mul_comm, <- Z.shiftl_mul_pow2, Shift.Z.testbit_add_shiftl_full; try lia.
+  - rewrite eval_cons, uweight_eval_shift
+      by (specialize (Hz a (or_introl eq_refl)); lia).
+    rewrite uweight_0, uweight_eq_alt', Z.mul_1_l, Z.mul_1_r, Z.mul_comm, <- Z.shiftl_mul_pow2, Shift.Z.testbit_add_shiftl_full
+      by (specialize (Hz a (or_introl eq_refl)); lia).
     destruct (m <? machine_wordsize) eqn:E.
     + rewrite Z.ltb_lt in E; rewrite Z.div_small by lia.
       rewrite ListUtil.nth_default_cons, Z.mod_small by lia. reflexivity.
@@ -199,8 +135,7 @@ Proof.
       replace machine_wordsize with (1 * machine_wordsize) at 1 by ring.
       rewrite Div.Z.div_sub, Z.sub_1_r, Z.succ_pred; lia.
       apply Div.Z.div_nonneg; lia.
-      intros; specialize (Hz z); tauto.
-    + specialize (Hz a (or_introl eq_refl)); lia. Qed.
+      intros; specialize (Hz z); tauto. Qed.
 
 (**************************************************** *)
 (**Functional correctness of multi-limb logical shift *)
@@ -216,7 +151,7 @@ Proof.
   generalize dependent n. induction f; intros; subst.
   - unfold sat_shiftr; simpl; rewrite eval0; reflexivity.
   - unfold sat_shiftr; simpl.
-    rewrite eval_cons, uweight_eval_shift; try lia.
+    rewrite eval_cons, uweight_eval_shift by lia.
     destruct f; simpl in *.
     + rewrite
         eval_cons, uweight_0, eval0, ListUtil.nth_default_cons, uweight_eq_alt',
@@ -239,8 +174,8 @@ Proof.
            rewrite Z.mul_1_r, Z.land_div2; rewrite ?Z.sub_simpl_r; lia.
         ** now rewrite Z.mul_0_r, Z.land_0_r.
       * unfold sat_shiftr. replace (S (length f) - 1)%nat with (length f) by omega.
-        apply app_split.
-        ** apply map_seq_ext; intros; try lia.
+        apply f_equal2.
+        ** apply map_seq_ext; intros; [|lia].
            rewrite Nat.sub_0_r, Nat.add_1_r.
            rewrite !(ListUtil.nth_default_cons_S _ a); reflexivity.
         ** now rewrite ListUtil.nth_default_cons_S. Qed.
@@ -277,23 +212,20 @@ Lemma sat_add_bounds machine_wordsize n f g
       (Hg : length g = n) :
   forall z, In z (sat_add machine_wordsize n f g) -> 0 <= z < 2 ^ machine_wordsize.
 Proof.
-  intros. unfold sat_add in *.
-  rewrite Rows.add_partitions in *; auto.
-  unfold Partition.partition in H.
-  apply ListAux.in_map_inv in H.
-  destruct H as [a [H]].
-  rewrite H0, !uweight_eq_alt; try lia.
-  split.
+  pose proof uwprops machine_wordsize mw0.
+  intros z Hin; unfold sat_add in *; rewrite Rows.add_partitions in *; auto.
+  unfold Partition.partition in Hin. apply ListAux.in_map_inv in Hin.
+  destruct Hin as [a [Hin]].
+  rewrite H0, !uweight_eq_alt by lia. split.
   - apply Z.div_le_lower_bound;
       ring_simplify; try apply Z.mod_pos_bound;
-        apply Z.pow_pos_nonneg; try lia; apply Z.pow_pos_nonneg; lia.
+        apply Z.pow_pos_nonneg; try apply Z.pow_pos_nonneg; lia.
   - apply Z.div_lt_upper_bound.
-    apply Z.pow_pos_nonneg; try lia; apply Z.pow_pos_nonneg; lia.
+    apply Z.pow_pos_nonneg; try apply Z.pow_pos_nonneg; lia.
     replace ((_ ^ _) ^ _ * _) with ((2 ^ machine_wordsize) ^ Z.of_nat (S a)).
-    apply Z.mod_pos_bound; apply Z.pow_pos_nonneg; try lia; apply Z.pow_pos_nonneg; lia.
-    rewrite Z.mul_comm, Pow.Z.pow_mul_base; 
-    try (replace (Z.of_nat (S a)) with ((Z.of_nat a + 1)) by lia; lia).
-  - apply (uwprops machine_wordsize mw0). Qed.
+    apply Z.mod_pos_bound; apply Z.pow_pos_nonneg; try apply Z.pow_pos_nonneg; lia.
+    rewrite Z.mul_comm, Pow.Z.pow_mul_base;
+    try (replace (Z.of_nat (S a)) with ((Z.of_nat a + 1)) by lia; lia). Qed.
 
 (********************************************************* *)
 (**Section on properties of sat_mod2 including correctness *)
@@ -318,27 +250,28 @@ Proof.
     rewrite Zmod_0_l, Z.add_0_r; reflexivity. Qed.
 
 (*********************************************************************** *)
-(**Section for properties of sat_arithmetic_shiftr including correctness *)
+(**Section for properties of sat_arithmetic_shiftr1 including correctness *)
 (*********************************************************************** *)
 
-Lemma eval_sat_arithmetic_shiftr machine_wordsize n f
+Lemma eval_sat_arithmetic_shiftr1 machine_wordsize n f
       (mw0 : 0 < machine_wordsize)
       (Hz : forall z, In z f -> 0 <= z < 2^machine_wordsize)
       (Hf : length f = n) :
-  eval (uweight machine_wordsize) n (sat_arithmetic_shiftr machine_wordsize n f) =
-  Z.arithmetic_shiftr (machine_wordsize * n) (eval (uweight machine_wordsize) n f).
+  eval (uweight machine_wordsize) n (sat_arithmetic_shiftr1 machine_wordsize n f) =
+  Z.arithmetic_shiftr1 (machine_wordsize * n) (eval (uweight machine_wordsize) n f).
 Proof.
   generalize dependent n.
   induction f as [|z f IHf]; intros; subst.
   - rewrite !eval0; reflexivity.
   - destruct f.
     + cbn; rewrite uweight_0, !Z.mul_1_r, !Z.mul_1_l, !Z.add_0_r; reflexivity.
-    + unfold sat_arithmetic_shiftr; simpl.
-      rewrite eval_cons, !uweight_eval_shift by (try lia; autorewrite with distr_length; reflexivity).
-      replace (map _ _ ++ _) with (sat_arithmetic_shiftr machine_wordsize (S (length f)) (z0 :: f)).
+    + unfold sat_arithmetic_shiftr1; simpl.
+      rewrite eval_cons, !uweight_eval_shift by (autorewrite with distr_length; try reflexivity; lia).
+      replace (map _ _ ++ _) with (sat_arithmetic_shiftr1 machine_wordsize (S (length f)) (z0 :: f)).
       rewrite IHf; try reflexivity.
 
-      unfold Z.arithmetic_shiftr; rewrite !Z.land_pow2_testbit, !eval_testbit; try tauto; try nia; simpl.
+      unfold Z.arithmetic_shiftr1.
+      rewrite !Z.land_pow2_testbit, !eval_testbit; try tauto; try nia; simpl.
       replace (Z.abs_nat ((machine_wordsize * Z.pos (Pos.succ (Pos.of_succ_nat (length f))) - 1) / machine_wordsize)) with
           (S (Z.abs_nat ((machine_wordsize * Z.pos (Pos.of_succ_nat (length f)) - 1) / machine_wordsize))).
       rewrite !ListUtil.nth_default_cons_S, !ListUtil.nth_default_cons by lia.
@@ -359,38 +292,40 @@ Proof.
         replace (machine_wordsize + (_ + _)) with
             (machine_wordsize * Z.pos (Pos.succ (Pos.of_succ_nat (length f))) + - (1)) by lia; ring.
 
-        rewrite Z.land_comm, Z.land_pow2_small; try lia.
+        rewrite Z.land_comm, Z.land_pow2_small; [lia|].
         split.
         apply Div.Z.div_nonneg; try lia.
            assert (0 <= eval (uweight machine_wordsize) (S (S (length f))) (z :: z0 :: f)).
            { apply eval_bound; try lia. intros; apply Hz; simpl; tauto. reflexivity. }
            specialize (Hz z (or_introl eq_refl)); nia.
-        apply Div.Z.div_lt_upper_bound'; try lia.
+        apply Div.Z.div_lt_upper_bound'; [lia|].
            rewrite Z.mul_comm, Pow.Z.pow_mul_base by nia.
         simpl; rewrite <- Z.add_assoc, Z.add_0_r.
         apply eval_bound; try lia; tauto.
 
-        rewrite Z.land_comm, Z.land_pow2_small; try lia.
+        rewrite Z.land_comm, Z.land_pow2_small; [lia|].
         split.
-        apply Div.Z.div_nonneg; try lia.
-        apply eval_bound; try lia. intros; apply Hz; simpl; tauto. reflexivity.
+        apply Div.Z.div_nonneg; [|lia].
+        apply eval_bound; [lia| |]. intros; apply Hz; simpl; tauto. reflexivity.
 
         apply Div.Z.div_lt_upper_bound'; try lia.
-        rewrite Z.mul_comm, Pow.Z.pow_mul_base; try nia. rewrite <- Z.add_assoc, Z.add_0_r.
-        apply eval_bound; try lia. intros; apply Hz; simpl; tauto. reflexivity.
+        rewrite Z.mul_comm, Pow.Z.pow_mul_base by nia. rewrite <- Z.add_assoc, Z.add_0_r.
+        apply eval_bound; try assumption. intros; apply Hz; simpl; tauto. reflexivity.
 
         rewrite Zmod_odd.
         specialize (Hz z (or_introl eq_refl)).
         destruct (Z.odd z0).
-        ** rewrite Z.mul_1_r, Z.land_pow2_small; try lia. split.
+        ** rewrite Z.mul_1_r, Z.land_pow2_small; [reflexivity|]. split.
            apply Div.Z.div_nonneg; lia.
-           apply Div.Z.div_lt_upper_bound'; try lia.
+           apply Div.Z.div_lt_upper_bound'; [lia|].
            rewrite Z.mul_comm, Pow.Z.pow_mul_base, Z.sub_simpl_r; lia.
         ** rewrite Z.mul_0_r, Z.land_0_r; reflexivity.
-      * rewrite !Z.lor_0_l, (eval_cons _ (S _)), uweight_eval_shift; try lia; try reflexivity.
+      * rewrite !Z.lor_0_l, (eval_cons _ (S _)), uweight_eval_shift
+          by (try reflexivity; lia).
         rewrite uweight_0, uweight_eq_alt', Z.mul_1_l, Z.mul_1_r.
         rewrite <- !Z.div2_spec, !Z.div2_div, Z.div2_split by lia.
-        rewrite eval_sat_mod2, sat_mod2_cons, Z.lor_add; try lia ; try reflexivity.
+        rewrite eval_sat_mod2, sat_mod2_cons, Z.lor_add;
+          [reflexivity| |reflexivity|lia].
         rewrite Zmod_odd. specialize (Hz z (or_introl eq_refl)).
         destruct (Z.odd z0).
         ** rewrite Z.mul_1_r, Z.land_pow2_small; try lia.
@@ -408,7 +343,7 @@ Proof.
         set (a := machine_wordsize). apply Div.Z.div_nonneg; nia.
       * intros; apply Hz; simpl in *; tauto.
       * intros; apply Hz; simpl in *; tauto.
-      * unfold sat_arithmetic_shiftr.
+      * unfold sat_arithmetic_shiftr1.
         replace (S (length f) - 1)%nat with (length f) by lia.
         rewrite ListUtil.nth_default_cons_S.
         apply f_equal2; [|reflexivity].
@@ -455,8 +390,8 @@ Proof. unfold sat_opp; rewrite length_sat_add; auto with distr_length. Qed.
 Hint Rewrite length_sat_opp : distr_length.
 
 Lemma eval_sat_opp machine_wordsize n f
-      (Hn : (0 < n)%nat)
       (mw0 : 0 < machine_wordsize)
+      (Hn : (0 < n)%nat)
       (Hz : forall z, In z f -> 0 <= z < 2^machine_wordsize)
       (Hf : length f = n) :
   eval (uweight machine_wordsize) n (sat_opp machine_wordsize n f) =
@@ -474,28 +409,28 @@ Proof.
 
     rewrite !eval_cons, uweight_0, !uweight_eval_shift, uweight_eq_alt' by distr_length.
     rewrite !Z.mul_1_l, !Z.mul_1_r, Z.opp_add_distr, Zopp_mult_distr_r, <- Z.add_mod_idemp_r by distr_length.
-    symmetry. rewrite Z.add_assoc, <- Z.add_mod_idemp_r; try (rewrite Zpos_P_of_succ_nat in H0; rewrite Nat2Z.inj_succ; assumption). 
+    symmetry. rewrite Z.add_assoc, <- Z.add_mod_idemp_r; try (rewrite Zpos_P_of_succ_nat in H0; rewrite Nat2Z.inj_succ; assumption).
     replace (2 ^ (machine_wordsize * Z.of_nat (S (length f)))) with
         ((2 ^ machine_wordsize) * (2 ^ (machine_wordsize * Z.of_nat (length f)))).
-    rewrite !Z.mul_mod_distr_l; try lia.
+    rewrite !Z.mul_mod_distr_l by lia.
     unfold Z.lnot_modulo. rewrite Lnot.Z.lnot_equiv. unfold Z.pred.
     destruct (length f) eqn:E.
     + rewrite !eval0.
       rewrite !Z.mul_0_r, !Z.mul_1_r, !Z.add_0_r.
       replace (-a + -1) with (- (a + 1)) by ring.
-      rewrite eval_sat_one by lia.
+      rewrite eval_sat_one.
       rewrite Z.mod_opp_small.
       replace (1 + (2 ^ machine_wordsize - (a + 1))) with
           (-a + 2 ^ machine_wordsize) by ring.
       rewrite <- Z.add_mod_idemp_r.
       rewrite Z_mod_same_full. rewrite Z.add_0_r. reflexivity.
       apply Z.pow_nonzero. omega. lia.
-      specialize (Hz a (or_introl eq_refl)). lia. 
-    + rewrite IHf; try lia.
-      rewrite !eval_sat_one in *; try lia; try apply uweight_0.
-      rewrite <- Z.mul_mod_distr_l, Z.add_mod_idemp_r; try nia.
+      specialize (Hz a (or_introl eq_refl)). lia. lia. lia.
+    + rewrite IHf by (try (intros; apply Hz; right; assumption); lia).
+      rewrite !eval_sat_one in * by lia.
+      rewrite <- Z.mul_mod_distr_l, Z.add_mod_idemp_r by nia.
       symmetry.
-      rewrite <- Z.mul_mod_distr_l, Z.add_mod_idemp_r, Z.mul_add_distr_l, Z.mul_1_r; try nia.
+      rewrite <- Z.mul_mod_distr_l, Z.add_mod_idemp_r, Z.mul_add_distr_l, Z.mul_1_r by nia.
       replace (-a + -1) with (- (a + 1)) by ring.
       rewrite Z.mod_opp_small.
       unfold Z.lnot_modulo.
@@ -504,7 +439,6 @@ Proof.
           (- a + 2 ^ machine_wordsize) by ring.
       reflexivity.
       specialize (Hz a (or_introl eq_refl)); lia.
-      intros; apply Hz; right; assumption.
     + rewrite <- Z.pow_add_r; try apply f_equal; nia. Qed.
 
 Lemma sat_opp_mod2 machine_wordsize n f
@@ -527,44 +461,30 @@ Proof.
 (**Properties of twos_complement_opp *)
 (*********************************** *)
 
+Lemma twos_complement_opp_bound m a (Hm : 0 <= m) :
+  0 <= Z.twos_complement_opp m a < 2 ^ m.
+Proof. unfold Z.twos_complement_opp; apply Z.mod_pos_bound.
+       apply Z.pow_pos_nonneg; lia. Qed.
+
 Lemma twos_complement_opp_correct m a :
   (Z.twos_complement_opp m a) = - a mod 2 ^ m.
+Proof. unfold Z.twos_complement_opp, Z.lnot_modulo, Z.lnot.
+       rewrite Zplus_mod_idemp_l, <- Z.sub_1_r; apply f_equal2; lia. Qed.
+
+Lemma twos_complement_zopp a m
+      (Hm : 0 < m) (corner_case : Z.twos_complement m a <> - 2 ^ (m - 1)) :
+  Z.twos_complement m (- a) = - Z.twos_complement m a.
 Proof.
-  unfold Z.twos_complement_opp.
-  unfold Z.lnot_modulo, Z.lnot.
-  rewrite Zplus_mod_idemp_l.
-  rewrite Z.add_1_r. rewrite Z.succ_pred. reflexivity. Qed.
-
-Lemma twosc_Z_opp a m
-      (Hm : 0 < m) (corner_case : twosc m a <> - 2 ^ (m - 1)) :
-  - twosc m a = twosc m (- a).
-Proof.
-  pose proof twosc_bounds a m Hm.
-
-  assert (0 < 2 ^ (m - 1)) by (apply Z.pow_pos_nonneg; lia).
-  assert (2 ^ m = 2 * 2 ^ (m - 1))
-    by (rewrite Pow.Z.pow_mul_base, Z.sub_simpl_r; lia).
-  assert (0 <= a mod 2 ^ m < 2 ^ m) by (apply Z.mod_pos_bound; lia).
-
-  destruct (dec (a mod 2 ^ m = 2 ^ (m - 1)));
-    destruct (dec (a mod 2 ^ m = 0)); rewrite ?e, ?e0; try lia.
-  - rewrite e, Z.ltb_irrefl in *. lia.
-  - rewrite PullPush.Z.opp_mod_mod, e, Z.mod_0_l by lia.
-    replace (0 <? 2 ^ (m - 1)) with true by (symmetry; apply Z.ltb_lt; lia); reflexivity.
-  - pose proof (mod_less_than_half_iff_not_neg_mod_less _ _ Hm n n0). symmetry in H3.
-    destruct (a mod 2 ^ m <? 2 ^ (m - 1)).
-    + apply negb_true_iff in H3; rewrite H3.
-      apply Z.ltb_ge in H3. rewrite PullPush.Z.opp_mod_mod, Z.mod_opp_small; lia.
-    + apply negb_false_iff in H3; rewrite H3.
-      apply Z.ltb_lt in H3. rewrite PullPush.Z.opp_mod_mod, Z.mod_opp_small; lia. Qed.
+  pose proof Z.twos_complement_bounds a m Hm.
+  apply Z.twos_complement_spec; [lia|split]; [|lia].
+  rewrite (PullPush.Z.opp_mod_mod (Z.twos_complement _ _)), Z.twos_complement_mod' by lia;
+    apply PullPush.Z.opp_mod_mod. Qed.
 
 Lemma twos_complement_opp_spec m a
-      (Hm : 0 < m)
-      (corner_case : twosc m a <> - 2 ^ (m - 1)) :
-  twosc m (Z.twos_complement_opp m a) = - (twosc m a).
-Proof.
-  unfold Z.twos_complement_opp, Z.lnot_modulo, Z.lnot.
-  rewrite Zplus_mod_idemp_l, Z.add_1_r, Z.succ_pred, twosc_mod by lia. symmetry; apply twosc_Z_opp; lia. Qed.
+      (Hm : 0 < m) (corner_case : Z.twos_complement m a <> - 2 ^ (m - 1)) :
+  Z.twos_complement m (Z.twos_complement_opp m a) = - (Z.twos_complement m a).
+Proof. apply Z.twos_complement_spec; [lia|split]; [|pose proof Z.twos_complement_bounds a m Hm; lia].
+       rewrite <- twos_complement_zopp, twos_complement_opp_correct, Z.twos_complement_mod', Z.mod_mod by (try apply Z.pow_nonzero; lia). reflexivity. Qed.
 
 (************************* *)
 (**Properties of twos_complement_pos *)
@@ -572,234 +492,77 @@ Proof.
 
 Lemma twos_complement_pos_spec m a
       (mw0 : 0 < m)
-      (corner_case : twosc m a <> - 2 ^ (m - 1)) : (* note that this has to be true for Z.twos_complement_pos to work *)
-  Z.twos_complement_pos m a = Z.b2z (0 <? twosc m a).
+      (corner_case : Z.twos_complement m a <> - 2 ^ (m - 1)) : (* note that this has to be true for Z.twos_complement_pos to work *)
+  Z.twos_complement_pos m a = Z.b2z (0 <? Z.twos_complement m a).
 Proof.
-  assert (0 < 2 ^ m) by (apply Z.pow_pos_nonneg; lia).
-  assert (0 <= a mod 2 ^ m < 2 ^ m) by (apply Z.mod_pos_bound; lia).
-  assert (2 ^ m = 2 * 2 ^ (m - 1)) by (rewrite Pow.Z.pow_mul_base; ring_simplify (m - 1 + 1); lia).
-
-  unfold Z.twos_complement_pos; cbv [Let_In]; rewrite twos_complement_opp_correct.
-  destruct (a mod 2 ^ m <? 2 ^ (m - 1)) eqn:E; destruct (dec (a mod 2 ^ m = 0)).
-  - rewrite PullPush.Z.opp_mod_mod, e; simpl; rewrite Z.mod_0_l, Z.shiftr_0_l; auto.
-    apply Z.pow_nonzero; lia.
-  - rewrite mod_less_than_half_iff_not_neg_mod_less in E; auto.
-    assert (0 <? a mod 2 ^ m = true) by (apply Z.ltb_lt; lia).
-    rewrite H2, Z.shiftr_div_pow2, Div.Z.div_between_1; try lia; auto.
-    rewrite negb_true_iff, Z.ltb_ge in E.
-    split; try lia.
-    rewrite H1. apply Z.mod_pos_bound; lia. rewrite Z.ltb_lt in E; lia.
-  - rewrite PullPush.Z.opp_mod_mod, e, !Z.mod_0_l, Z.shiftr_0_l; try lia.
-    assert (0 <? 0 - 2 ^ m = false) by (apply Z.ltb_ge; lia). rewrite H2; reflexivity.
-  - rewrite mod_less_than_half_iff_not_neg_mod_less in E; try lia; auto.
-    assert (0 <? a mod 2 ^ m - 2 ^ m = false) by (apply Z.ltb_ge; lia).
-    rewrite H2, Z.shiftr_div_pow2, Z.div_small; try lia; auto.
-    rewrite negb_false_iff, Z.ltb_lt in E. split; try apply Z.mod_pos_bound; lia. Qed.
-
-(****************************************************************************** *)
-(**This section is for the interaction between twosc and integer addition       *)
-(**There are some badly named lemmas. These are just casing on some inequalites *)
-(**of the sum of to numbers under modular reduction.                            *)
-(****************************************************************************** *)
-
-Lemma mod_add a b m
-      (Hm : 0 < m)
-      (Ha : a mod 2 ^ m < (2 ^ (m - 1)))
-      (Hb : b mod 2 ^ m < (2 ^ (m - 1))) :
-  (a + b) mod 2 ^ m = a mod 2 ^ m + b mod 2 ^ m.
-Proof.
-  assert (0 < 2 ^ m) by (apply Z.pow_pos_nonneg; lia).
-  assert (0 <= a mod 2 ^ m) by (apply Z.mod_pos_bound; lia).
-  assert (0 <= b mod 2 ^ m) by (apply Z.mod_pos_bound; lia).
-
-  rewrite <- Zplus_mod_idemp_l, <- Zplus_mod_idemp_r.
-  rewrite Z.mod_small. lia. replace (2 ^ m) with (2 * 2 ^ (m - 1)) at 5. lia.
-  rewrite Pow.Z.pow_mul_base, Z.sub_simpl_r; lia. Qed.
-
-Lemma mod_add2 a b m
-      (Hm : 0 < m)
-      (Ha : a mod 2 ^ m < (2 ^ (m - 1)))
-      (Hb : 2 ^ (m - 1) <= b mod 2 ^ m)
-      (Hsum : (a + b) mod 2 ^ m < 2 ^ (m - 1)) :
-  (a + b) mod 2 ^ m = a mod 2 ^ m + b mod 2 ^ m - 2 ^ m.
-Proof.
-  assert (0 < 2 ^ m) by (apply Z.pow_pos_nonneg; lia).
-  assert (0 <= a mod 2 ^ m < 2 ^ m) by (apply Z.mod_pos_bound; lia).
-  assert (0 <= b mod 2 ^ m < 2 ^ m) by (apply Z.mod_pos_bound; lia).
-  assert (2 ^ m <= a mod 2 ^ m + b mod 2 ^ m < 2 * 2 ^ m).
-  { split; try lia.
-    destruct (dec (2 ^ m <= a mod 2 ^ m + b mod 2 ^ m)); try lia.
-    apply Znot_le_gt in n. rewrite <- Zplus_mod_idemp_l, <- Zplus_mod_idemp_r, Z.mod_small in Hsum; lia. }
-  rewrite <- Zplus_mod_idemp_l, <- Zplus_mod_idemp_r, Modulo.Z.mod_small_1; lia. Qed.
-
-Lemma mod_add3 a b m
-      (Hm : 0 < m)
-      (Ha : a mod 2 ^ m < (2 ^ (m - 1)))
-      (Hb : 2 ^ (m - 1) <= b mod 2 ^ m)
-      (Hsum : 2 ^ (m - 1) <= (a + b) mod 2 ^ m) :
-  (a + b) mod 2 ^ m = a mod 2 ^ m + b mod 2 ^ m.
-Proof.
-  assert (0 < 2 ^ m) by (apply Z.pow_pos_nonneg; lia).
-  assert (0 <= a mod 2 ^ m < 2 ^ m) by (apply Z.mod_pos_bound; lia).
-  assert (0 <= b mod 2 ^ m < 2 ^ m) by (apply Z.mod_pos_bound; lia).
-
-  assert (0 <= a mod 2 ^ m + b mod 2 ^ m < 2 ^ m).
-  split; try lia.
-  destruct (dec (a mod 2 ^ m + b mod 2 ^ m < 2 ^ m)); try lia.
-  apply Znot_lt_ge in n.
-  rewrite <- Zplus_mod_idemp_l, <- Zplus_mod_idemp_r, Modulo.Z.mod_small_1 in Hsum; lia.
-  rewrite <- Zplus_mod_idemp_l, <- Zplus_mod_idemp_r, Z.mod_small; lia. Qed.
-
-Lemma mod_add4 a b m
-      (Hm : 0 < m)
-      (Ha : 2 ^ (m - 1) <= a mod 2 ^ m)
-      (Hb : 2 ^ (m - 1) <= b mod 2 ^ m) :
-  (a + b) mod 2 ^ m = a mod 2 ^ m + b mod 2 ^ m - 2 ^ m.
-Proof.
-  assert (0 < 2 ^ m) by (apply Z.pow_pos_nonneg; lia).
-  assert (0 <= a mod 2 ^ m < 2 ^ m) by (apply Z.mod_pos_bound; lia).
-  assert (0 <= b mod 2 ^ m < 2 ^ m) by (apply Z.mod_pos_bound; lia).
-
-  assert (2 ^ m = 2 * 2 ^ (m - 1))
-    by (rewrite Pow.Z.pow_mul_base, Z.sub_simpl_r; lia).
-
-  rewrite <- Zplus_mod_idemp_l, <- Zplus_mod_idemp_r, Modulo.Z.mod_small_1; lia. Qed.
-
-Lemma twosc_add a b m
-      (Hm : 0 < m)
-      (Ha : - 2 ^ (m - 2) < twosc m a < 2 ^ (m - 2))
-      (Hb : - 2 ^ (m - 2) < twosc m b < 2 ^ (m - 2)) :
-  twosc m (a + b) = twosc m a + twosc m b.
-Proof.
-  destruct (dec (m = 1)).
-  rewrite e in *; replace (2 ^ (1 - 2)) with 0 in * by reflexivity; lia.
-
-  assert (0 < 2 ^ m) by (apply Z.pow_pos_nonneg; lia).
-  assert (2 ^ m = 2 * 2 ^ (m - 1))
-    by (rewrite Pow.Z.pow_mul_base, Z.sub_simpl_r; lia).
-  assert (2 ^ m = 2 * (2 * 2 ^ (m - 2)))
-    by (rewrite !Pow.Z.pow_mul_base; replace (m - 2 + 1 + 1) with m by ring; lia).
-
-  assert (0 <= a mod 2 ^ m < 2 ^ m) by (apply Z.mod_pos_bound; lia).
-  assert (0 <= b mod 2 ^ m < 2 ^ m) by (apply Z.mod_pos_bound; lia).
-
-  destruct ((a + b) mod 2 ^ m <? 2 ^ (m - 1)) eqn:Hsum;
-    destruct (a mod 2 ^ m <? 2 ^ (m - 1)) eqn:Hamod;
-    destruct (b mod 2 ^ m <? 2 ^ (m - 1)) eqn:Hbmod;
-    rewrite ?Z.ltb_lt, ?Z.ltb_ge in *.
-  - apply mod_add; lia.
-  - rewrite Z.add_sub_assoc. apply mod_add2; lia.
-  - rewrite Z.add_comm, <- Z.add_sub_swap.
-    rewrite (Z.add_comm (a mod _)). apply mod_add2; try lia. rewrite Z.add_comm; lia.
-  - assert (2 ^ m <= a mod 2 ^ m + b mod 2 ^ m < 2 * 2 ^ m) by (split; lia).
-    rewrite <- Zplus_mod_idemp_l, <- Zplus_mod_idemp_r, Modulo.Z.mod_small_1 in Hsum; lia.
-  - rewrite <- Zplus_mod_idemp_l, <- Zplus_mod_idemp_r, Z.mod_small in Hsum; lia.
-  - rewrite mod_add3; lia.
-  - rewrite Z.add_comm, mod_add3; try lia. rewrite Z.add_comm; lia.
-  - rewrite mod_add4; lia. Qed.
-
-Lemma mod_add_full a b m
-      (Hm : 0 < m)
-      (Hsum : a mod m + b mod m < m) :
-  (a + b) mod m = a mod m + b mod m.
-Proof.
-  assert (0 <= a mod m < m) by (apply Z.mod_pos_bound; lia).
-  assert (0 <= b mod m < m) by (apply Z.mod_pos_bound; lia).
-  rewrite <- Zplus_mod_idemp_l, <- Zplus_mod_idemp_r, Z.mod_small; lia. Qed.
-
-Lemma twosc_add_full a b m
-      (Hm : 0 < m)
-      (Ha : - 2 ^ (m - 1) <= twosc m a + twosc m b < 2 ^ (m - 1)) :
-  twosc m (a + b) = twosc m a + twosc m b.
-Proof.
-  assert (0 < 2 ^ m) by (apply Z.pow_pos_nonneg; lia).
-  assert (2 ^ m = 2 * 2 ^ (m - 1))
-    by (rewrite Pow.Z.pow_mul_base, Z.sub_simpl_r; lia).
-
-  assert (0 <= a mod 2 ^ m < 2 ^ m) by (apply Z.mod_pos_bound; lia).
-  assert (0 <= b mod 2 ^ m < 2 ^ m) by (apply Z.mod_pos_bound; lia).
-
-  destruct ((a + b) mod 2 ^ m <? 2 ^ (m - 1)) eqn:Hsum;
-    destruct (a mod 2 ^ m <? 2 ^ (m - 1)) eqn:Hamod;
-    destruct (b mod 2 ^ m <? 2 ^ (m - 1)) eqn:Hbmod;
-    rewrite ?Z.ltb_lt, ?Z.ltb_ge in *.
-  - rewrite mod_add_full; lia.
-  - rewrite mod_add2; lia.
-  - rewrite Z.add_comm. rewrite <- Z.add_sub_swap.
-    rewrite (Z.add_comm (a mod _)). apply mod_add2. lia. lia. lia.
-    rewrite Z.add_comm; lia.
-  - assert (2 ^ m <= a mod 2 ^ m + b mod 2 ^ m < 2 * 2 ^ m) by (split; lia).
-    rewrite <- Zplus_mod_idemp_l, <- Zplus_mod_idemp_r, Modulo.Z.mod_small_1 in Hsum; lia.
-  - rewrite <- Zplus_mod_idemp_l, <- Zplus_mod_idemp_r, Z.mod_small in Hsum; lia.
-  - rewrite mod_add3; lia.
-  - rewrite Z.add_comm, mod_add3; try lia. rewrite Z.add_comm; lia.
-  - rewrite mod_add4; lia. Qed.
+  replace (0 <? Z.twos_complement m a) with (- Z.twos_complement m a <? 0) by
+      (destruct (0 <? Z.twos_complement m a) eqn:?; destruct (- Z.twos_complement m a <? 0) eqn:?;
+                rewrite ?Z.ltb_lt in *; rewrite ?Z.ltb_ge in *; try reflexivity; lia).
+  unfold Z.twos_complement_pos; pose proof twos_complement_opp_bound m a ltac:(lia).
+  rewrite <- twos_complement_opp_spec, unfold_Let_In, Z.twos_complement_neg_equiv by lia.
+  rewrite Z.sign_bit_testbit, Z.twos_complement_cond_equiv, negb_involutive; lia. Qed.
 
 (********************************************************************* *)
-(**Section for interaction between eval_twosc and saturated operations *)
+(**Section for interaction between eval_twos_complement and saturated operations *)
 (********************************************************************* *)
 
-Lemma eval_twosc_sat_arithmetic_shiftr machine_wordsize n f
+Lemma eval_twos_complement_sat_arithmetic_shiftr1 machine_wordsize n f
       (mw0 : 0 < machine_wordsize)
       (n0 : (0 < n)%nat)
       (Hz : forall z, In z f -> 0 <= z < 2^machine_wordsize)
       (Hf : length f = n) :
-  eval_twosc machine_wordsize n (sat_arithmetic_shiftr machine_wordsize n f) =
-  (eval_twosc machine_wordsize n f) / 2.
+  eval_twos_complement machine_wordsize n (sat_arithmetic_shiftr1 machine_wordsize n f) =
+  (eval_twos_complement machine_wordsize n f) / 2.
 Proof.
-  assert (0 < Z.of_nat n) by omega. unfold eval_twosc. rewrite eval_sat_arithmetic_shiftr, arithmetic_shiftr_spec; auto; try nia.
+  assert (0 < Z.of_nat n) by omega. unfold eval_twos_complement. rewrite eval_sat_arithmetic_shiftr1, Z.arithmetic_shiftr1_spec; auto; [nia|].
   apply eval_bound; auto. Qed.
 
-Lemma eval_twosc_sat_add machine_wordsize n f g
+Lemma eval_twos_complement_sat_add machine_wordsize n f g
       (mw0 : 0 < machine_wordsize)
       (n0 : (0 < n)%nat)
       (Hf : length f = n)
       (Hg : length g = n)
       (overflow_f : - 2 ^ (machine_wordsize * n - 2) <
-                    twosc (machine_wordsize * n) (eval (uweight machine_wordsize) n f) <
+                    Z.twos_complement (machine_wordsize * n) (eval (uweight machine_wordsize) n f) <
                     2 ^ (machine_wordsize * n - 2))
       (overflow_g : - 2 ^ (machine_wordsize * n - 2) <
-                    twosc (machine_wordsize * n) (eval (uweight machine_wordsize) n g) <
+                    Z.twos_complement (machine_wordsize * n) (eval (uweight machine_wordsize) n g) <
                     2 ^ (machine_wordsize * n - 2)) :
-  eval_twosc machine_wordsize n (sat_add machine_wordsize n f g) =
-  eval_twosc machine_wordsize n f + eval_twosc machine_wordsize n g.
-Proof. assert (0 < Z.of_nat n) by omega. unfold eval_twosc. rewrite eval_sat_add, twosc_mod, twosc_add; nia. Qed.
+  eval_twos_complement machine_wordsize n (sat_add machine_wordsize n f g) =
+  eval_twos_complement machine_wordsize n f + eval_twos_complement machine_wordsize n g.
+Proof. assert (0 < Z.of_nat n) by omega; unfold eval_twos_complement.
+       rewrite eval_sat_add, <- Z.twos_complement_add_weak, Z.twos_complement_mod; lia. Qed.
 
-Lemma eval_twosc_select machine_wordsize n cond f g
+Lemma eval_twos_complement_select machine_wordsize n cond f g
       (Hf : length f = n)
       (Hg : length g = n) :
-  eval_twosc machine_wordsize n (select cond f g) = if dec (cond = 0)
-                                                    then (eval_twosc machine_wordsize n f)
-                                                    else (eval_twosc machine_wordsize n g).
-Proof. unfold eval_twosc; rewrite eval_select; auto; destruct (dec (cond = 0)); auto. Qed.
+  eval_twos_complement machine_wordsize n (select cond f g) = if dec (cond = 0)
+                                                    then (eval_twos_complement machine_wordsize n f)
+                                                    else (eval_twos_complement machine_wordsize n g).
+Proof. unfold eval_twos_complement; rewrite eval_select; auto; destruct (dec (cond = 0)); auto. Qed.
 
-Lemma eval_twosc_sat_opp machine_wordsize n f
+Lemma eval_twos_complement_sat_opp machine_wordsize n f
       (mw0 : 0 < machine_wordsize)
       (n0 : (0 < n)%nat)
       (Hz : forall z, In z f -> 0 <= z < 2^machine_wordsize)
       (Hf : length f = n)
-      (corner_case : eval_twosc machine_wordsize n f <> - 2 ^ (machine_wordsize * n - 1)):
-  eval_twosc machine_wordsize n (sat_opp machine_wordsize n f) =
-  - eval_twosc machine_wordsize n f.
-Proof. assert (0 < Z.of_nat n) by omega; unfold eval_twosc in *; rewrite eval_sat_opp, twosc_mod, twosc_Z_opp; try nia; tauto. Qed.
+      (corner_case : eval_twos_complement machine_wordsize n f <> - 2 ^ (machine_wordsize * n - 1)):
+  eval_twos_complement machine_wordsize n (sat_opp machine_wordsize n f) =
+  - eval_twos_complement machine_wordsize n f.
+Proof. assert (0 < Z.of_nat n) by omega; unfold eval_twos_complement in *; rewrite eval_sat_opp, Z.twos_complement_mod, twos_complement_zopp; try tauto; nia. Qed.
 
-Lemma eval_twosc_sat_zero machine_wordsize n
+Lemma eval_twos_complement_sat_zero machine_wordsize n
       (mw0 : 0 < machine_wordsize)
       (n0 : (0 < n)%nat) :
-  eval_twosc machine_wordsize n (sat_zero n) = 0.
-Proof.
-  unfold eval_twosc; rewrite eval_sat_zero; auto.
-  rewrite Z.mod_0_l by (apply Z.pow_nonzero; nia).
-  assert (0 <? 2 ^ (machine_wordsize * Z.of_nat n - 1) = true) by (apply Z.ltb_lt; apply Z.pow_pos_nonneg; nia).
-  now rewrite H. Qed.
+  eval_twos_complement machine_wordsize n (sat_zero n) = 0.
+Proof. unfold eval_twos_complement; rewrite eval_sat_zero by lia; apply Z.twos_complement_zero; nia. Qed.
 
-Lemma eval_twosc_sat_mod2 machine_wordsize n f
+Lemma eval_twos_complement_sat_mod2 machine_wordsize n f
       (mw0 : 0 < machine_wordsize)
       (n0 : (0 < n)%nat)
       (Hf : length f = n) :
-  (eval_twosc machine_wordsize n f) mod 2 = sat_mod2 f.
-Proof.
-  assert (0 < Z.of_nat n) by omega. unfold eval_twosc. rewrite twosc_mod2, eval_sat_mod2; nia. Qed.
+  (eval_twos_complement machine_wordsize n f) mod 2 = sat_mod2 f.
+Proof. unfold eval_twos_complement; rewrite Z.twos_complement_mod2, eval_sat_mod2; nia. Qed.
 
 (** ******************************************************************************* *)
 (** This section is for the implementation and correctness of the divstep algorithm *)
@@ -824,7 +587,7 @@ Definition divstep_aux machine_wordsize sat_limbs mont_limbs m (data : Z * (list
   dlet g0 := sat_mod2 g' in
   let d'' := (d' + 1) mod 2^machine_wordsize in
   dlet f'' := select g0 (sat_zero sat_limbs) f' in
-  let g'' := sat_arithmetic_shiftr machine_wordsize sat_limbs (sat_add machine_wordsize sat_limbs g' f'') in
+  let g'' := sat_arithmetic_shiftr1 machine_wordsize sat_limbs (sat_add machine_wordsize sat_limbs g' f'') in
   dlet v''' := select g0 (sat_zero mont_limbs) v' in
   let r'' := addmod machine_wordsize mont_limbs m r' v''' in
     (d'',f',g'',v'',r'').
@@ -853,24 +616,24 @@ Definition divstep_spec_full m d f g v r :=
 Lemma divstep_g machine_wordsize sat_limbs mont_limbs m d f g v r
       (mw0 : 0 < machine_wordsize)
       (sat_limbs0 : (0 < sat_limbs)%nat)
-      (fodd : Z.odd (eval_twosc machine_wordsize sat_limbs f) = true)
+      (fodd : Z.odd (eval_twos_complement machine_wordsize sat_limbs f) = true)
       (Hf : length f = sat_limbs)
       (Hg : length g = sat_limbs)
-      (corner_case : twosc machine_wordsize d <> - 2 ^ (machine_wordsize - 1))
+      (corner_case : Z.twos_complement machine_wordsize d <> - 2 ^ (machine_wordsize - 1))
       (overflow_f : - 2 ^ (machine_wordsize * sat_limbs - 2) <
-                    eval_twosc machine_wordsize sat_limbs f <
+                    eval_twos_complement machine_wordsize sat_limbs f <
                     2 ^ (machine_wordsize * sat_limbs - 2))
       (overflow_g : - 2 ^ (machine_wordsize * sat_limbs - 2) <
-                    eval_twosc machine_wordsize sat_limbs g <
+                    eval_twos_complement machine_wordsize sat_limbs g <
                     2 ^ (machine_wordsize * sat_limbs - 2))
       (Hf2 : forall z, In z f -> 0 <= z < 2^machine_wordsize)
       (Hg2 : forall z, In z g -> 0 <= z < 2^machine_wordsize) :
   let '(d1,f1,g1,v1,r1) := (divstep machine_wordsize sat_limbs mont_limbs m d f g v r) in
-  eval_twosc machine_wordsize sat_limbs g1 =
+  eval_twos_complement machine_wordsize sat_limbs g1 =
   snd (divstep_spec
-         (twosc machine_wordsize d)
-         (eval_twosc machine_wordsize sat_limbs f)
-         (eval_twosc machine_wordsize sat_limbs g)).
+         (Z.twos_complement machine_wordsize d)
+         (eval_twos_complement machine_wordsize sat_limbs f)
+         (eval_twos_complement machine_wordsize sat_limbs g)).
 Proof.
   set (bw := machine_wordsize * Z.of_nat sat_limbs) in *.
 
@@ -885,55 +648,55 @@ Proof.
 
   Hint Rewrite length_sat_add length_sat_opp length_select : distr_length.
 
-  rewrite eval_twosc_sat_arithmetic_shiftr; distr_length; autorewrite with distr_length; try nia.
-  rewrite eval_twosc_sat_add; auto; try (autorewrite with distr_length; lia).
-  rewrite !eval_twosc_select; auto; try (autorewrite with distr_length; lia).
-  rewrite eval_twosc_sat_opp; auto; try (autorewrite with distr_length; lia).
+  rewrite eval_twos_complement_sat_arithmetic_shiftr1; distr_length; autorewrite with distr_length; try nia.
+  rewrite eval_twos_complement_sat_add; auto; try (autorewrite with distr_length; lia).
+  rewrite !eval_twos_complement_select; auto; try (autorewrite with distr_length; lia).
+  rewrite eval_twos_complement_sat_opp; auto; try (autorewrite with distr_length; lia).
   rewrite select_push; try (autorewrite with distr_length; lia).
 
   rewrite sat_opp_mod2; auto.
   unfold divstep_spec.
   rewrite twos_complement_pos_spec; auto.
-  rewrite <- !(eval_twosc_sat_mod2 machine_wordsize sat_limbs); auto.
+  rewrite <- !(eval_twos_complement_sat_mod2 machine_wordsize sat_limbs); auto.
   rewrite !Zmod_odd; auto.
 
-  set (g' := eval_twosc machine_wordsize sat_limbs g) in *.
-  set (f' := eval_twosc machine_wordsize sat_limbs f) in *.
+  set (g' := eval_twos_complement machine_wordsize sat_limbs g) in *.
+  set (f' := eval_twos_complement machine_wordsize sat_limbs f) in *.
   assert (corner_case_f : f' <> - 2 ^ (bw - 1)) by
       (replace (- _) with (- (2 * 2 ^ (bw - 2))); rewrite ?Pow.Z.pow_mul_base; ring_simplify (bw - 2 + 1); nia).
 
-  destruct (0 <? twosc machine_wordsize d);
+  destruct (0 <? Z.twos_complement machine_wordsize d);
     destruct (Z.odd g') eqn:g'_odd; rewrite ?fodd, ?eval_sat_zero; auto.
-  - simpl. rewrite Z.add_comm; reflexivity.
-  - simpl. rewrite eval_twosc_sat_zero; auto.
-  - rewrite Z.mul_1_l. simpl. reflexivity.
-  - simpl. rewrite eval_twosc_sat_zero; auto.
-  - replace (_ * _) with bw by reflexivity. lia.
-  - fold (eval_twosc machine_wordsize sat_limbs
+  - simpl; rewrite Z.add_comm; reflexivity.
+  - simpl; rewrite eval_twos_complement_sat_zero; auto.
+  - rewrite Z.mul_1_l; simpl; reflexivity.
+  - simpl; rewrite eval_twos_complement_sat_zero; auto.
+  - replace (_ * _) with bw by reflexivity; lia.
+  - fold (eval_twos_complement machine_wordsize sat_limbs
                      (select (Z.twos_complement_pos machine_wordsize d &' sat_mod2 g) g (sat_opp machine_wordsize sat_limbs f))).
-    rewrite eval_twosc_select; try apply length_sat_opp; auto.
+    rewrite eval_twos_complement_select; try apply length_sat_opp; auto.
     destruct (dec (_)); replace (machine_wordsize * _) with bw by reflexivity;
-    try rewrite eval_twosc_sat_opp; auto; replace (machine_wordsize * _) with bw by reflexivity; lia.
-  - fold (eval_twosc machine_wordsize sat_limbs
+    try rewrite eval_twos_complement_sat_opp; auto; replace (machine_wordsize * _) with bw by reflexivity; lia.
+  - fold (eval_twos_complement machine_wordsize sat_limbs
                      (select (sat_mod2 (select (Z.twos_complement_pos machine_wordsize d &' sat_mod2 g) g (sat_opp machine_wordsize sat_limbs f)))
                              (sat_zero sat_limbs) (select (Z.twos_complement_pos machine_wordsize d &' sat_mod2 g) f g))).
-    rewrite eval_twosc_select; try apply length_sat_zero; try apply length_select; auto.
-    destruct (dec (_)); try rewrite eval_twosc_sat_zero; try rewrite eval_twosc_select;
+    rewrite eval_twos_complement_select; try apply length_sat_zero; try apply length_select; auto.
+    destruct (dec (_)); try rewrite eval_twos_complement_sat_zero; try rewrite eval_twos_complement_select;
       replace (machine_wordsize * _) with bw by reflexivity; try lia; destruct (dec (_)); lia.
-  - apply sat_add_bounds; try lia; repeat (rewrite ?length_sat_opp, ?(length_select sat_limbs), ?length_sat_zero; auto). Qed.
+  - apply sat_add_bounds; repeat (rewrite ?length_sat_opp, ?(length_select sat_limbs), ?length_sat_zero; auto); lia. Qed.
 
 Lemma divstep_d machine_wordsize sat_limbs mont_limbs m d f g v r
       (mw1 : 1 < machine_wordsize)
       (sat_limbs0 : (0 < sat_limbs)%nat)
       (Hg : length g = sat_limbs)
       (overflow_d : - 2 ^ (machine_wordsize - 1) + 1 <
-                    twosc machine_wordsize d <
+                    Z.twos_complement machine_wordsize d <
                     2 ^ (machine_wordsize - 1) - 1) :
   let '(d1,f1,g1,v1,r1) := (divstep machine_wordsize sat_limbs mont_limbs m d f g v r) in
-  twosc machine_wordsize d1 =
-  fst (fst (divstep_spec (twosc machine_wordsize d)
-                           (eval_twosc machine_wordsize sat_limbs f)
-                           (eval_twosc machine_wordsize sat_limbs g))).
+  Z.twos_complement machine_wordsize d1 =
+  fst (fst (divstep_spec (Z.twos_complement machine_wordsize d)
+                           (eval_twos_complement machine_wordsize sat_limbs f)
+                           (eval_twos_complement machine_wordsize sat_limbs g))).
 Proof.
   assert (helper0 : 0 < Z.of_nat sat_limbs) by omega.
   assert (mw0 : 0 < machine_wordsize) by lia.
@@ -943,72 +706,72 @@ Proof.
     by (rewrite Pow.Z.pow_mul_base, Z.sub_simpl_r; lia).
 
   simpl; unfold divstep_spec.
-  rewrite twos_complement_pos_spec, <- (eval_twosc_sat_mod2 machine_wordsize sat_limbs), Zmod_odd; auto; try nia.
-  fold (eval_twosc machine_wordsize sat_limbs g); set (g' := eval_twosc machine_wordsize sat_limbs g) in *.
-  destruct ((0 <? twosc machine_wordsize d) && (Z.odd g')) eqn:E.
+  rewrite twos_complement_pos_spec, <- (eval_twos_complement_sat_mod2 machine_wordsize sat_limbs), Zmod_odd by nia.
+  fold (eval_twos_complement machine_wordsize sat_limbs g); set (g' := eval_twos_complement machine_wordsize sat_limbs g) in *.
+  destruct ((0 <? Z.twos_complement machine_wordsize d) && (Z.odd g')) eqn:E.
   - apply andb_prop in E. destruct E; rewrite H, H0. simpl Z.b2z; simpl Z.land; cbv [fst].
     unfold Z.zselect. simpl (if _ =? _ then _ else _).
-    rewrite twos_complement_opp_correct, twosc_mod, twosc_add_full, twosc_mod, <- twosc_Z_opp, twosc_one; try lia.
-    rewrite twosc_mod, <- twosc_Z_opp, twosc_one; lia.
+    rewrite twos_complement_opp_correct, Z.twos_complement_mod, Z.twos_complement_add_full, Z.twos_complement_mod, twos_complement_zopp, Z.twos_complement_one; try lia.
+    rewrite Z.twos_complement_mod, twos_complement_zopp, Z.twos_complement_one; lia.
   - apply andb_false_iff in E.
     destruct E; rewrite H;
       unfold Z.zselect; cbv [fst]; simpl (if _ =? _ then _ else _);
         [destruct (Z.odd g') | rewrite Z.land_0_r; simpl (if _ =? _ then _ else _)];
-        rewrite twosc_mod, twosc_add_full, twosc_one; try rewrite ?twosc_one; lia. Qed.
+        rewrite Z.twos_complement_mod, Z.twos_complement_add_full, Z.twos_complement_one; rewrite ?Z.twos_complement_one; lia. Qed.
 
 Lemma divstep_f machine_wordsize sat_limbs mont_limbs m d f g v r
       (mw0 : 0 < machine_wordsize)
       (Hf : length f = sat_limbs)
       (Hg : length g = sat_limbs)
-      (corner_case : twosc machine_wordsize d <> - 2 ^ (machine_wordsize - 1)) :
+      (corner_case : Z.twos_complement machine_wordsize d <> - 2 ^ (machine_wordsize - 1)) :
   let '(d1,f1,g1,v1,r1) := (divstep machine_wordsize sat_limbs mont_limbs m d f g v r) in
-  eval_twosc machine_wordsize sat_limbs f1 =
-  snd (fst (divstep_spec (twosc machine_wordsize d)
-                           (eval_twosc machine_wordsize sat_limbs f)
-                           (eval_twosc machine_wordsize sat_limbs g))).
+  eval_twos_complement machine_wordsize sat_limbs f1 =
+  snd (fst (divstep_spec (Z.twos_complement machine_wordsize d)
+                           (eval_twos_complement machine_wordsize sat_limbs f)
+                           (eval_twos_complement machine_wordsize sat_limbs g))).
 Proof.
   destruct sat_limbs. subst.
-  unfold eval_twosc.
+  unfold eval_twos_complement.
   rewrite !eval0; rewrite Z.mul_0_r.
-  replace (twosc 0 0) with (-1). unfold divstep_spec.
-  destruct (0 <? twosc machine_wordsize d); reflexivity. reflexivity.
+  replace (Z.twos_complement 0 0) with (-1). unfold divstep_spec.
+  destruct (0 <? Z.twos_complement machine_wordsize d); reflexivity. reflexivity.
 
   unfold divstep_spec.
   simpl.
 
   set (n' := S sat_limbs) in *.
   assert (0 < n')%nat by apply Nat.lt_0_succ.
-  rewrite eval_twosc_select, twos_complement_pos_spec, <- (eval_twosc_sat_mod2 machine_wordsize n'), Zmod_odd; auto.
-  fold (eval_twosc machine_wordsize n' g).
-  destruct (0 <? twosc machine_wordsize d); destruct (Z.odd (eval_twosc machine_wordsize n' g));
+  rewrite eval_twos_complement_select, twos_complement_pos_spec, <- (eval_twos_complement_sat_mod2 machine_wordsize n'), Zmod_odd; auto.
+  fold (eval_twos_complement machine_wordsize n' g).
+  destruct (0 <? Z.twos_complement machine_wordsize d); destruct (Z.odd (eval_twos_complement machine_wordsize n' g));
     try reflexivity; lia. Qed.
 
 Theorem divstep_correct machine_wordsize sat_limbs mont_limbs m d f g v r
         (mw1 : 1 < machine_wordsize)
         (sat_limbs0 : (0 < sat_limbs)%nat)
-        (fodd : Z.odd (eval_twosc machine_wordsize sat_limbs f) = true)
+        (fodd : Z.odd (eval_twos_complement machine_wordsize sat_limbs f) = true)
         (Hf : length f = sat_limbs)
         (Hg : length g = sat_limbs)
         (overflow_d : - 2 ^ (machine_wordsize - 1) + 1 <
-                    twosc machine_wordsize d <
+                    Z.twos_complement machine_wordsize d <
                     2 ^ (machine_wordsize - 1) - 1)
         (overflow_f : - 2 ^ (machine_wordsize * sat_limbs - 2) <
-                      eval_twosc machine_wordsize sat_limbs f <
+                      eval_twos_complement machine_wordsize sat_limbs f <
                       2 ^ (machine_wordsize * sat_limbs - 2))
         (overflow_g : - 2 ^ (machine_wordsize * sat_limbs - 2) <
-                      eval_twosc machine_wordsize sat_limbs g <
+                      eval_twos_complement machine_wordsize sat_limbs g <
                       2 ^ (machine_wordsize * sat_limbs - 2))
         (Hf2 : forall z, In z f -> 0 <= z < 2^machine_wordsize)
         (Hg2 : forall z, In z g -> 0 <= z < 2^machine_wordsize) :
   let '(d1,f1,g1,v1,r1) := (divstep machine_wordsize sat_limbs mont_limbs m d f g v r) in
-  (twosc machine_wordsize d1,
-   eval_twosc machine_wordsize sat_limbs f1,
-   eval_twosc machine_wordsize sat_limbs g1) =
-  divstep_spec (twosc machine_wordsize d)
-               (eval_twosc machine_wordsize sat_limbs f)
-               (eval_twosc machine_wordsize sat_limbs g).
+  (Z.twos_complement machine_wordsize d1,
+   eval_twos_complement machine_wordsize sat_limbs f1,
+   eval_twos_complement machine_wordsize sat_limbs g1) =
+  divstep_spec (Z.twos_complement machine_wordsize d)
+               (eval_twos_complement machine_wordsize sat_limbs f)
+               (eval_twos_complement machine_wordsize sat_limbs g).
 Proof.
-  assert (0 < machine_wordsize) by lia.
+  assert (0 < machine_wordsize) by lia. simpl.
   apply injective_projections.
   apply injective_projections.
   rewrite <- (divstep_d _ _ mont_limbs m _ _ _ v r); auto.
@@ -1016,7 +779,7 @@ Proof.
   rewrite <- (divstep_g _ _ mont_limbs m _ _ _ v r); auto; lia. Qed.
 
 Lemma divstep_v machine_wordsize sat_limbs mont_limbs m (r' : Z) m' d f g v r
-      (fodd : Z.odd (eval_twosc machine_wordsize sat_limbs f) = true)
+      (fodd : Z.odd (eval_twos_complement machine_wordsize sat_limbs f) = true)
 
       (r'_correct : (2 ^ machine_wordsize * r') mod m = 1)
       (m'_correct : (m * m') mod 2 ^ machine_wordsize = -1 mod 2 ^ machine_wordsize)
@@ -1031,13 +794,13 @@ Lemma divstep_v machine_wordsize sat_limbs mont_limbs m (r' : Z) m' d f g v r
       (Hr : length r = mont_limbs)
       (Hg : length g = sat_limbs)
       (overflow_d : - 2 ^ (machine_wordsize - 1) + 1 <
-                    twosc machine_wordsize d <
+                    Z.twos_complement machine_wordsize d <
                     2 ^ (machine_wordsize - 1) - 1) :
   let '(d1,f1,g1,v1,r1) := (divstep machine_wordsize sat_limbs mont_limbs m d f g v r) in
   @WordByWordMontgomery.eval machine_wordsize mont_limbs
                         (from_montgomerymod machine_wordsize mont_limbs m m' v1) mod m =
-  fst (divstep_spec2 m (twosc machine_wordsize d)
-                (eval_twosc machine_wordsize sat_limbs g)
+  fst (divstep_spec2 m (Z.twos_complement machine_wordsize d)
+                (eval_twos_complement machine_wordsize sat_limbs g)
                 (@WordByWordMontgomery.eval machine_wordsize mont_limbs
                                        (from_montgomerymod machine_wordsize mont_limbs m m' v))
                 (@WordByWordMontgomery.eval machine_wordsize mont_limbs
@@ -1046,11 +809,11 @@ Proof.
   assert (sat_limbs <> 0%nat) by lia.
   assert (mont_limbs <> 0%nat) by lia.
   simpl.
-  rewrite twos_complement_pos_spec, <- (eval_twosc_sat_mod2 machine_wordsize sat_limbs) by lia.
+  rewrite twos_complement_pos_spec, <- (eval_twos_complement_sat_mod2 machine_wordsize sat_limbs) by lia.
   rewrite Zmod_odd, (select_eq (uweight machine_wordsize) _ mont_limbs); auto.
   unfold divstep_spec2.
-  destruct (0 <? twosc machine_wordsize d);
-    destruct (Z.odd (eval_twosc machine_wordsize sat_limbs g));
+  destruct (0 <? Z.twos_complement machine_wordsize d);
+    destruct (Z.odd (eval_twos_complement machine_wordsize sat_limbs g));
     rewrite ?(eval_addmod _ _ _ r'), ?Z.add_diag; auto. Qed.
 
 Lemma nonzero_zero n :
@@ -1063,10 +826,10 @@ Lemma zero_valid machine_wordsize n m
   valid machine_wordsize n m (sat_zero n).
 Proof.
   unfold valid, small, WordByWordMontgomery.eval.
-  rewrite eval_sat_zero, partition_0; try split; auto; try lia. Qed.
+  rewrite eval_sat_zero, partition_0; try split; auto; lia. Qed.
 
 Lemma divstep_r machine_wordsize sat_limbs mont_limbs m (r' : Z) m' d f g v r
-      (fodd : Z.odd (eval_twosc machine_wordsize sat_limbs f) = true)
+      (fodd : Z.odd (eval_twos_complement machine_wordsize sat_limbs f) = true)
       (r'_correct : (2 ^ machine_wordsize * r') mod m = 1)
       (m'_correct : (m * m') mod 2 ^ machine_wordsize = -1 mod 2 ^ machine_wordsize)
       (m_big : 1 < m)
@@ -1081,14 +844,14 @@ Lemma divstep_r machine_wordsize sat_limbs mont_limbs m (r' : Z) m' d f g v r
       (Hf : length f = sat_limbs)
       (Hg : length g = sat_limbs)
       (overflow_d : - 2 ^ (machine_wordsize - 1) + 1 <
-                    twosc machine_wordsize d <
+                    Z.twos_complement machine_wordsize d <
                     2 ^ (machine_wordsize - 1) - 1)
       (Hf2 : forall z, In z f -> 0 <= z < 2^machine_wordsize) :
   let '(d1,f1,g1,v1,r1) := (divstep machine_wordsize sat_limbs mont_limbs m d f g v r) in
   @WordByWordMontgomery.eval machine_wordsize mont_limbs
                         (from_montgomerymod machine_wordsize mont_limbs m m' r1) mod m =
-  snd (divstep_spec2 m (twosc machine_wordsize d)
-                (eval_twosc machine_wordsize sat_limbs g)
+  snd (divstep_spec2 m (Z.twos_complement machine_wordsize d)
+                (eval_twos_complement machine_wordsize sat_limbs g)
                 (@WordByWordMontgomery.eval machine_wordsize mont_limbs
                                        (from_montgomerymod machine_wordsize mont_limbs m m' v))
                 (@WordByWordMontgomery.eval machine_wordsize mont_limbs
@@ -1102,16 +865,17 @@ Proof.
   destruct H as [H1 H2].
   assert (zero_valid : valid machine_wordsize mont_limbs m (sat_zero mont_limbs)) by (apply zero_valid; lia).
   pose proof (nonzero_zero mont_limbs) as H3.
-  rewrite (nonzeromod_correct machine_wordsize mont_limbs m r' m') in H3; try apply zero_valid; try lia; auto.
+  rewrite (nonzeromod_correct machine_wordsize mont_limbs m r' m') in H3
+    by (try apply zero_valid; lia).
 
   simpl.
   rewrite select_push; rewrite ?length_sat_opp; auto.
   rewrite sat_opp_mod2; auto.
-  rewrite twos_complement_pos_spec, <- !(eval_twosc_sat_mod2 machine_wordsize sat_limbs); try lia.
+  rewrite twos_complement_pos_spec, <- !(eval_twos_complement_sat_mod2 machine_wordsize sat_limbs) by lia.
   rewrite !Zmod_odd, !(select_eq (uweight machine_wordsize) _ mont_limbs), fodd;
     try apply length_select; auto.
-  destruct (0 <? twosc machine_wordsize d);
-    destruct (Z.odd (eval_twosc machine_wordsize sat_limbs g)); simpl.
+  destruct (0 <? Z.twos_complement machine_wordsize d);
+    destruct (Z.odd (eval_twos_complement machine_wordsize sat_limbs g)); simpl.
   - rewrite (eval_addmod _ _ _ r'); auto.
     rewrite <- Zplus_mod_idemp_l; auto.
     rewrite (eval_oppmod _ _ _ r'); auto.
@@ -1171,7 +935,7 @@ Proof. unfold divstep_spec2, divstep_spec_full.
        destruct ((0 <? d) && Z.odd g); reflexivity. Qed.
 
 Theorem divstep_correct_full machine_wordsize sat_limbs mont_limbs m r' m' d f g v r
-      (fodd : Z.odd (eval_twosc machine_wordsize sat_limbs f) = true)
+      (fodd : Z.odd (eval_twos_complement machine_wordsize sat_limbs f) = true)
       (r'_correct : (2 ^ machine_wordsize * r') mod m = 1)
       (m'_correct : (m * m') mod 2 ^ machine_wordsize = -1 mod 2 ^ machine_wordsize)
       (m_big : 1 < m)
@@ -1184,27 +948,27 @@ Theorem divstep_correct_full machine_wordsize sat_limbs mont_limbs m r' m' d f g
       (Hf : length f = sat_limbs)
       (Hg : length g = sat_limbs)
       (overflow_d : - 2 ^ (machine_wordsize - 1) + 1 <
-                    twosc machine_wordsize d <
+                    Z.twos_complement machine_wordsize d <
                     2 ^ (machine_wordsize - 1) - 1)
       (overflow_f : - 2 ^ (machine_wordsize * sat_limbs - 2) <
-                    eval_twosc machine_wordsize sat_limbs f <
+                    eval_twos_complement machine_wordsize sat_limbs f <
                     2 ^ (machine_wordsize * sat_limbs - 2))
       (overflow_g : - 2 ^ (machine_wordsize * sat_limbs - 2) <
-                    eval_twosc machine_wordsize sat_limbs g <
+                    eval_twos_complement machine_wordsize sat_limbs g <
                     2 ^ (machine_wordsize * sat_limbs - 2))
       (Hf2 : forall z, In z f -> 0 <= z < 2^machine_wordsize)
       (Hg2 : forall z, In z g -> 0 <= z < 2^machine_wordsize)
       (Hv2 : valid machine_wordsize mont_limbs m v)
       (Hr2 : valid machine_wordsize mont_limbs m r) :
   let '(d1,f1,g1,v1,r1) := (divstep machine_wordsize sat_limbs mont_limbs m d f g v r) in
-    (twosc machine_wordsize d1,
-     eval_twosc machine_wordsize sat_limbs f1,
-     eval_twosc machine_wordsize sat_limbs g1,
+    (Z.twos_complement machine_wordsize d1,
+     eval_twos_complement machine_wordsize sat_limbs f1,
+     eval_twos_complement machine_wordsize sat_limbs g1,
      @WordByWordMontgomery.eval machine_wordsize mont_limbs (from_montgomerymod machine_wordsize mont_limbs m m' v1) mod m,
      @WordByWordMontgomery.eval machine_wordsize mont_limbs (from_montgomerymod machine_wordsize mont_limbs m m' r1) mod m) =
-    divstep_spec_full m (twosc machine_wordsize d)
-                      (eval_twosc machine_wordsize sat_limbs f)
-                      (eval_twosc machine_wordsize sat_limbs g)
+    divstep_spec_full m (Z.twos_complement machine_wordsize d)
+                      (eval_twos_complement machine_wordsize sat_limbs f)
+                      (eval_twos_complement machine_wordsize sat_limbs g)
                       (@WordByWordMontgomery.eval machine_wordsize mont_limbs (from_montgomerymod machine_wordsize mont_limbs m m' v))
                       (@WordByWordMontgomery.eval machine_wordsize mont_limbs (from_montgomerymod machine_wordsize mont_limbs m m' r)).
 Proof.
