src/Util/ZUtil/SignBit.v
@@ -1,0 +1,64 @@
+Require Import Coq.Bool.Bool.
+Require Import Coq.ZArith.ZArith.
+Require Import Coq.micromega.Lia.
+
+Require Import Crypto.Util.ZUtil.Definitions.
+Require Import Crypto.Util.ZUtil.Notations.
+Require Import Crypto.Util.ZUtil.Land.
+Require Import Crypto.Util.ZUtil.Testbit.
+Require Import Crypto.Util.ZUtil.TwosComplement.
+
+Require Import Crypto.Util.ZUtil.Tactics.SolveRange.
+
+Import Notations.
+
+Local Open Scope Z_scope.
+
+Module Z.
+  Lemma sign_bit_0_land_pow2 a m :
+    Z.sign_bit m a = 0 -> a &' 2 ^ (m - 1) = 0.
+  Proof.
+    intros H; apply Z.shiftr_eq_0_iff in H; destruct H as [? |[? ?] ]; subst.
+    - rewrite Z.land_0_l; reflexivity.
+    - rewrite Z.land_pow2_testbit, Z.bits_above_log2; lia. Qed.
+
+  Lemma sign_bit_testbit a m
+        (Hm : 0 < m)
+        (H : 0 <= a < 2 ^ m) :
+    Z.sign_bit m a = Z.b2z (Z.testbit a (m - 1)).
+  Proof.
+    rewrite Z.testbit_spec', Z.mod_small, <- Z.shiftr_div_pow2 by solve_range.
+    reflexivity. Qed.
+
+  Lemma sign_bit_equiv a m
+        (Hm : 0 < m)
+        (Ha : 0 <= a < 2 ^ m) :
+    Z.sign_bit m a = Z.b2z (negb (a <? 2 ^ (m - 1))).
+  Proof. rewrite <- (Z.mod_small _ _ Ha) at 2.
+         rewrite Z.twos_complement_cond_equiv, sign_bit_testbit, negb_involutive; lia. Qed.
+
+  Lemma sign_bit_1_land_pow2 a m
+        (Hm : 0 < m)
+        (Ha : 0 <= a < 2 ^ m) :
+    Z.sign_bit m a <> 0 -> a &' 2 ^ (m - 1) = 2 ^ (m - 1).
+  Proof.
+    intros H. rewrite Z.land_pow2_testbit, Z.testbit_b2z, <- sign_bit_testbit by assumption.
+    apply Z.eqb_neq in H; rewrite H; reflexivity. Qed.
+
+  Lemma sign_bit_0_testbit a m
+        (Hm : 0 < m) :
+    Z.sign_bit m a = 0 -> Z.testbit a (m - 1) = false.
+  Proof.
+    assert (Hnz : 2 ^ (m - 1) <> 0) by (apply Z.pow_nonzero; lia).
+    intro H; apply sign_bit_0_land_pow2 in H. rewrite Z.land_pow2_testbit in H;
+                                                destruct (Z.testbit a (m - 1));
+                                                [contradiction|reflexivity]. Qed.
+
+  Lemma sign_bit_1_testbit a m
+        (Hm : 0 < m)
+        (Ha : 0 <= a < 2 ^ m) :
+    Z.sign_bit m a <> 0 -> Z.testbit a (m - 1) = true.
+  Proof.
+    rewrite Z.testbit_b2z, <- sign_bit_testbit by lia; intro H.
+    apply Z.eqb_neq in H; rewrite H; reflexivity. Qed.
+End Z.
