src/Util/ZUtil/TruncatingShiftl.v
@@ -3,6 +3,8 @@ Require Import Coq.micromega.Lia.
 Require Import Crypto.Util.ZUtil.Definitions.
 Require Import Crypto.Util.ZUtil.Notations.
 Require Import Crypto.Util.ZUtil.Pow.
+Require Import Crypto.Util.ZUtil.Modulo.
+Require Import Crypto.Util.ZUtil.Tactics.BruteForceIneq.
 Local Open Scope Z_scope.
 
 Module Z.
@@ -31,4 +33,61 @@ Module Z.
     unfold Definitions.Z.truncating_shiftl. rewrite Z.shiftl_mul_pow2 by lia.
     replace (2^b) with (2 * 2^(b-1)) by (rewrite Pow.Z.pow_mul_base, Z.sub_simpl_r; lia).
     rewrite Zmult_mod_distr_r; ring. Qed.
+
+  Lemma truncating_shiftl_testbit_spec m a k i
+        (Hm : 0 <= m)
+        (Hi : 0 <= i) :
+    Z.testbit (Z.truncating_shiftl m a k) i
+    = if (i <? m) then Z.testbit a (i - k) else false.
+  Proof.
+    unfold Z.truncating_shiftl. brute_force_ineq.
+    rewrite Z.mod_pow2_bits_low; try lia; apply Z.shiftl_spec; lia.
+    rewrite Z.mod_pow2_bits_high; try lia; reflexivity. Qed.
+
+  Lemma truncating_shiftl_truncating_shiftl m a p q
+        (Hp : 0 <= p)
+        (Hq : 0 <= q) :
+    Z.truncating_shiftl m (Z.truncating_shiftl m a p) q
+    = Z.truncating_shiftl m a (p + q).
+  Proof.
+    destruct (Z_lt_dec m 0).
+    { unfold Z.truncating_shiftl; rewrite Z.pow_neg_r, !Zmod_0_r;
+        [reflexivity|assumption]. }
+    apply Z.bits_inj'; intros i Hi.
+    rewrite truncating_shiftl_testbit_spec by lia.
+    destruct (Z_lt_dec (i - q) 0).
+    - rewrite Z.testbit_neg_r, truncating_shiftl_testbit_spec, Z.testbit_neg_r by lia;
+      brute_force_ineq.
+    - rewrite !truncating_shiftl_testbit_spec; brute_force_ineq; apply f_equal2; lia. Qed.
+
+  Lemma truncating_shiftl0 m k :
+    Z.truncating_shiftl m 0 k = 0.
+  Proof. unfold Z.truncating_shiftl. rewrite Z.shiftl_0_l, Zmod_0_l; reflexivity. Qed.
+
+  Lemma truncating_shiftl_lor m a b k :
+    Z.truncating_shiftl m (a |' b) k
+    = (Z.truncating_shiftl m a k) |' (Z.truncating_shiftl m b k).
+  Proof.
+    unfold Z.truncating_shiftl.
+    destruct (Z_lt_dec m 0).
+    - rewrite Z.pow_neg_r, !Zmod_0_r by assumption. reflexivity.
+    - rewrite <- !Z.land_ones, Z.shiftl_lor, Z.land_lor_distr_l by lia. reflexivity. Qed.
+
+  Lemma truncating_shiftl_large m a k (Hk : k >= m) :
+    Z.truncating_shiftl m a k = 0.
+  Proof.
+    unfold Z.truncating_shiftl.
+    destruct (Z_lt_dec m 0).
+    - rewrite Z.pow_neg_r, !Zmod_0_r by assumption; reflexivity.
+    - rewrite Z.shiftl_mul_pow2.
+      rewrite <- Zmult_mod_idemp_r, Z.mod_same_pow.
+      rewrite Z.mul_0_r. reflexivity. lia. lia. Qed.
+
+  Lemma truncating_shiftl_range m a k (Hm : 0 <= m) :
+    0 <= Z.truncating_shiftl m a k < 2 ^ m.
+  Proof. unfold Z.truncating_shiftl; apply Z.mod_pos_bound; apply Z.pow_pos_nonneg; lia. Qed.
+
+  Lemma truncating_shiftl_nonneg m a k (Hm : 0 <= m) :
+    0 <= Z.truncating_shiftl m a k.
+  Proof. unfold Z.truncating_shiftl; apply Z.mod_pos_bound; apply Z.pow_pos_nonneg; lia. Qed.
 End Z.
