src/Util/ZUtil/TwosComplement.v
@@ -1,0 +1,145 @@
+Require Import Coq.Bool.Bool.
+Require Import Coq.ZArith.ZArith.
+Require Import Coq.micromega.Lia.
+
+Require Import Crypto.Util.ZUtil.Definitions.
+Require Import Crypto.Util.ZUtil.Pow.
+Require Import Crypto.Util.ZUtil.Testbit.
+Require Import Crypto.Util.ZUtil.Modulo.
+Require Import Crypto.Util.ZUtil.Lor.
+Require Import Crypto.Util.ZUtil.Notations.
+
+Require Import Crypto.Util.ZUtil.Tactics.PullPush.
+Require Import Crypto.Util.ZUtil.Tactics.SolveTestbit.
+Require Import Crypto.Util.Tactics.BreakMatch.
+Require Import Crypto.Util.ZUtil.Tactics.LtbToLt.
+
+Require Import Crypto.Util.Decidable.
+
+Import Notations.
+
+Local Open Scope Z_scope.
+
+Module Z.
+  Local Ltac destruct_ltb a b :=
+    let E := fresh in
+    destruct (a <? b) eqn:E; [rewrite Z.ltb_lt in E|rewrite Z.ltb_ge in E].
+  Local Ltac destruct_leb a b :=
+    let E := fresh in
+    destruct (a <=? b) eqn:E; [rewrite Z.leb_le in E|rewrite Z.leb_gt in E].
+  Local Ltac destruct_eqb a b :=
+    let E := fresh in
+    destruct (a =? b) eqn:E; [rewrite Z.eqb_eq in E|rewrite Z.eqb_neq in E].
+
+  Lemma twos_complement_neg_equiv m a
+    (Hm : 0 < m) :
+    Z.twos_complement m a <? 0 = negb (a mod 2 ^ m <? 2 ^ (m - 1)).
+  Proof.
+    assert (0 < 2 ^ m) by (apply Z.pow_pos_nonneg; lia).
+    assert (0 <= a mod 2 ^ m < 2 ^ m) by (apply Z.mod_pos_bound; lia).
+    unfold Z.twos_complement. Z.ltb_to_lt; break_match; try discriminate; lia. Qed.
+
+  Lemma twos_complement_cond_equiv m a
+        (Hm : 0 < m) :
+    (a mod 2 ^ m) <? 2 ^ (m - 1) = negb (Z.testbit a (m - 1)).
+  Proof.
+    pose proof Z.mod_pos_bound a (2 ^ m) ltac:(apply Z.pow_pos_nonneg;lia).
+    destruct_ltb (a mod 2 ^ m) (2 ^ (m - 1)).
+    rewrite <- (Z.mod_pow2_bits_low _ m) by lia.
+    destruct (dec (a mod 2 ^ m = 0)) as [amod0|]; rewrite ?amod0, ?Z.bits_0, ?Z.bits_above_log2; try reflexivity.
+    apply Z.mod_pos_bound; lia. apply Z.log2_lt_pow2; lia.
+    rewrite <- (Z.mod_pow2_bits_low _ m),  Z.testbit_large by lia; reflexivity. Qed.
+
+  Lemma twos_complement_spec m a b
+    (Hm : 0 < m) :
+    Z.twos_complement m a = b <-> a mod 2 ^ m = b mod 2 ^ m /\ - 2 ^ (m - 1) <= b < 2 ^ (m - 1).
+  Proof.
+    unfold Z.twos_complement.
+    assert (0 < 2 ^ m) by (apply Z.pow_pos_nonneg; lia).
+    assert (0 <= a mod 2 ^ m < 2 ^ m) by (apply Z.mod_pos_bound; lia).
+    assert (2 ^ (m - 1) <= 2 ^ m) by (apply Z.pow_le_mono_r; lia).
+    assert (2 * 2 ^ (m - 1) = 2 ^ m) by (rewrite Z.pow_mul_base by lia; apply f_equal2; lia).
+    split; destruct_ltb (a mod 2 ^ m) (2 ^ (m - 1)); intros H4; subst; try split;
+      repeat (pull_Zmod; push_Zmod; rewrite ?Z.mod_0_l, ?Z.sub_0_r); try lia.
+    - destruct H4. rewrite H4 in *. rewrite Z.mod_small. lia.
+      destruct (dec (b < 0)); [|lia]. pose proof Z.mod_neg_small b (2 ^ m) ltac:(nia).
+      rewrite Z.mod_small in H6; lia.
+    - destruct H4. rewrite H4 in *. rewrite Z.mod_neg_small. lia.
+      destruct (dec (0 <= b)); [|lia]. rewrite Z.mod_small in H3; lia. Qed.
+
+  Lemma twos_complement_testbit_spec m a i
+        (Hi : 0 <= i)
+        (Hm : 0 < m) :
+    Z.testbit (Z.twos_complement m a) i = if (i <? m) then Z.testbit a i else Z.testbit a (m - 1).
+  Proof. unfold Z.twos_complement. unfold Z.sub at 2.
+         rewrite <- Z.lor_add by solve_using_testbit.
+         rewrite Z.twos_complement_cond_equiv by assumption.
+         destruct (Z.testbit a (m - 1)); solve_testbit. Qed.
+
+  Hint Rewrite twos_complement_testbit_spec : testbit_rewrite.
+
+  Lemma twos_complement_one m (Hm : 1 < m) :
+    Z.twos_complement m 1 = 1.
+  Proof.
+    apply twos_complement_spec; try split; try lia.
+    assert (1 < 2 ^ (m - 1)) by (apply Zpow_facts.Zpower_gt_1; lia); lia. Qed.
+
+  Lemma twos_complement_zero m (Hm : 0 < m):
+    Z.twos_complement m 0 = 0.
+  Proof. assert (0 < 2 ^ m) by (apply Z.pow_pos_nonneg; lia).
+         assert (0 < 2 ^ (m - 1)) by (apply Z.pow_pos_nonneg; lia).
+         apply twos_complement_spec; try split; rewrite ?Z.mod_0_l; lia. Qed.
+
+  Lemma twos_complement_mod a m (Hm : 0 < m) :
+    Z.twos_complement m (a mod 2 ^ m) = Z.twos_complement m a.
+  Proof. unfold Z.twos_complement; rewrite Z.mod_mod; try apply Z.pow_nonzero; lia. Qed.
+
+  Lemma twos_complement_mod' a m (Hm : 0 < m) :
+    Z.twos_complement m a mod 2 ^ m = a mod 2 ^ m.
+  Proof. unfold Z.twos_complement.
+         destruct_ltb (a mod 2 ^ m) (2 ^ (m - 1)); repeat (pull_Zmod; push_Zmod; rewrite Z.mod_0_l, Z.sub_0_r);
+           try apply Z.mod_mod; apply Z.pow_nonzero; lia. Qed.
+
+  Lemma twos_complement_odd m a (Hm : 0 < m) : Z.odd (Z.twos_complement m a) = Z.odd a.
+  Proof. rewrite <- !Z.bit0_odd. solve_testbit. Qed.
+
+  Lemma twos_complement_mod2 m a (Hm : 0 < m) : Z.twos_complement m a mod 2 = a mod 2.
+  Proof. rewrite Zmod_odd, twos_complement_odd, <- Zmod_odd by lia. reflexivity. Qed.
+
+  Lemma twos_complement_bounds a m (Hm : 0 < m) :
+    - 2 ^ (m - 1) <= Z.twos_complement m a < 2 ^ (m - 1).
+  Proof.
+    unfold Z.twos_complement.
+    assert (0 < 2 ^ m) by (apply Z.pow_pos_nonneg; lia).
+    assert (2 ^ m = 2 * 2 ^ (m - 1)) by (rewrite Z.pow_mul_base by lia; apply f_equal2; lia).
+    pose proof (Z.mod_pos_bound a (2 ^ m) H); destruct_ltb (a mod 2 ^ m) (2 ^ (m - 1)); lia. Qed.
+
+  Hint Resolve twos_complement_bounds : zarith.
+
+  Lemma twos_complement_add_full a b m
+      (Hm : 0 < m)
+      (Hsum : - 2 ^ (m - 1) <= Z.twos_complement m a + Z.twos_complement m b < 2 ^ (m - 1)) :
+    Z.twos_complement m (a + b) = Z.twos_complement m a + Z.twos_complement m b.
+  Proof.
+    apply twos_complement_spec; try split; try lia; unfold Z.twos_complement.
+    destruct_ltb (a mod 2 ^ m) (2 ^ (m - 1));
+      destruct_ltb (b mod 2 ^ m) (2 ^ (m - 1)); repeat (push_Zmod; pull_Zmod; rewrite ?Z.sub_0_r); reflexivity. Qed.
+
+  Lemma twos_complement_add_weak a b m
+        (Hm : 0 < m)
+        (Ha : - 2 ^ (m - 2) <= Z.twos_complement m a < 2 ^ (m - 2))
+        (Hb : - 2 ^ (m - 2) <= Z.twos_complement m b < 2 ^ (m - 2)) :
+    Z.twos_complement m (a + b) = Z.twos_complement m a + Z.twos_complement m b.
+  Proof. destruct (dec (m = 1)); [subst; rewrite Z.pow_neg_r in *; lia|].
+         assert (2 * 2 ^ (m - 2) = 2 ^ (m - 1)) by (rewrite Z.pow_mul_base by lia; apply f_equal2; lia).
+         rewrite twos_complement_add_full; lia. Qed.
+
+  Lemma twos_complement_mul_full m a b
+        (Hm : 0 < m)
+        (Hprod : - 2 ^ (m - 1) <= Z.twos_complement m a * Z.twos_complement m b < 2 ^ (m - 1)) :
+    Z.twos_complement m (a * b) = Z.twos_complement m a * Z.twos_complement m b.
+  Proof.
+    apply twos_complement_spec; try split; try lia; unfold Z.twos_complement.
+    destruct_ltb (a mod 2 ^ m) (2 ^ (m - 1));
+      destruct_ltb (b mod 2 ^ m) (2 ^ (m - 1)); repeat (push_Zmod; pull_Zmod; rewrite ?Z.sub_0_r); reflexivity. Qed.
+End Z.
